Support structs/unions with named fields in frontend.

frontend.v
@@ -1,6 +1,7 @@
 (* Copyright (c) 2012-2014, Robbert Krebbers. *)
 (* This file is distributed under the terms of the BSD license. *)
 Require Import type_system expression_eval.
+Require Import nmap.
 Local Open Scope expr_scope.
 Local Open Scope ctype_scope.
 
@@ -22,7 +23,7 @@ Inductive cexpr (Ti : Set) : Set :=
   | EAnd : cexpr Ti → cexpr Ti → cexpr Ti
   | EOr : cexpr Ti → cexpr Ti → cexpr Ti
   | ECast : type Ti → cexpr Ti → cexpr Ti
-  | EField : cexpr Ti → nat → cexpr Ti.
+  | EField : cexpr Ti → N → cexpr Ti.
 Arguments EVar {_} _.
 Arguments EConst {_} _ _.
 Arguments ESizeOf {_} _.
@@ -69,7 +70,7 @@ Arguments SWhile {_} _ _.
 Arguments SIf {_} _ _ _.
 
 Inductive decl (Ti : Set) : Set :=
-  | CompoundDecl : list (type Ti) → decl Ti
+  | CompoundDecl : list (N * type Ti) → decl Ti
   | GlobDecl : type Ti → option (cexpr Ti) → decl Ti
   | FunDecl : list (N * type Ti) → type Ti → cstmt Ti → decl Ti.
 Arguments CompoundDecl {_} _.
@@ -77,6 +78,14 @@ Arguments GlobDecl {_} _ _.
 Arguments FunDecl {_} _ _ _.
 
 Notation var_env Ti := (list (N * (index + type Ti))).
+Notation rename_env := (tagmap (list N)).
+
+Definition find_index {A} (P : A → Prop)
+    `{∀ x, Decision (P x)} : nat → list A → option nat :=
+  fix go i l :=
+  match l with
+  | [] => None | x :: l => if decide (P x) then Some i else go (S i) l
+  end.
 
 Section frontend.
 Context `{IntEnv Ti, PtrEnv Ti}.
@@ -101,7 +110,7 @@ Definition to_R (eτlr : expr Ti * lrtype Ti) : expr Ti * type Ti :=
     end
   | (e, inr τ) => (e,τ)
   end%E.
-Definition to_expr (Γ : env Ti) (Γf : funtypes Ti) (m : mem Ti)
+Definition to_expr (Γn : rename_env) (Γ : env Ti) (Γf : funtypes Ti) (m : mem Ti)
     (xs : var_env Ti) : cexpr Ti → option (expr Ti * lrtype Ti) :=
   fix go ce :=
   match ce with
@@ -178,11 +187,12 @@ Definition to_expr (Γ : env Ti) (Γf : funtypes Ti) (m : mem Ti)
      '(e,τ) ← to_R <$> go ce;
      guard (cast_typed Γ τ σ);
      Some (cast{σ} e, inr σ)
-  | EField ce i =>
+  | EField ce x =>
      '(e,τrl) ← go ce;
      τ ← maybe_inl τrl;
      '(c,s) ← maybe_TCompound τ;
      σs ← Γ !! s;
+     i ← Γn !! s ≫= find_index (x =) 0;
      σ ← σs !! i;
      Some (e .> i, inl σ)
   end%E.
@@ -232,11 +242,11 @@ Definition to_while (e : expr Ti) (con bre : bool) (Ls : labelset) :
   | false, false =>
      (Ls, None, None, λ s, while{e} s)
   end.
-Definition alloc_global (Γ : env Ti) (m : mem Ti) (xs : var_env Ti) (x : N)
-    (τ : type Ti) (mce : option (cexpr Ti)) : option (mem Ti * var_env Ti) :=
+Definition alloc_global (Γn : rename_env) (Γ : env Ti) (m : mem Ti) (xs : var_env Ti)
+    (x : N) (τ : type Ti) (mce : option (cexpr Ti)) : option (mem Ti * var_env Ti) :=
   match mce with
   | Some ce =>
-     '(e,τ') ← to_R <$> to_expr Γ ∅ m xs ce;
+     '(e,τ') ← to_R <$> to_expr Γn Γ ∅ m xs ce;
      guard (τ = τ');
      guard (int_typed (size_of Γ τ) sptrT);
      v ← ⟦ e ⟧ Γ ∅ [] m ≫= maybe_inr;
@@ -250,20 +260,20 @@ Definition alloc_global (Γ : env Ti) (m : mem Ti) (xs : var_env Ti) (x : N)
            (x,inl o) :: xs)
   end.
 
-Definition to_stmt (Γ : env Ti) (Γf : funtypes Ti) :
+Definition to_stmt (Γn : rename_env) (Γ : env Ti) (Γf : funtypes Ti) :
     mem Ti → var_env Ti → labelset → option labelname → option labelname →
     cstmt Ti → option (mem Ti * stmt Ti * rettype Ti) :=
   fix go m xs Ls mLc mLb cs {struct cs} :=
   match cs with
   | SDo ce =>
-     '(e,_) ← to_R <$> to_expr Γ Γf m xs ce;
+     '(e,_) ← to_R <$> to_expr Γn Γ Γf m xs ce;
      Some (m, !e, (false, None))
   | SSkip => Some (m, skip, (false, None))
   | SGoto l => Some (m, goto l, (true, None))
   | SContinue => Lc ← mLc; Some (m, goto Lc, (true, None))
   | SBreak => Lb ← mLb; Some (m, goto Lb, (true, None))
   | SReturn (Some ce) =>
-     '(e,τ) ← to_R <$> to_expr Γ Γf m xs ce;
+     '(e,τ) ← to_R <$> to_expr Γn Γ Γf m xs ce;
      Some (m, ret e, (true, Some τ))
   | SReturn None => Some (m, ret (#voidV), (true, Some voidT))
   | SBlock x τ None cs =>
@@ -274,12 +284,12 @@ Definition to_stmt (Γ : env Ti) (Γf : funtypes Ti) :
   | SBlock x τ (Some ce) cs =>
      guard (✓{Γ} τ);
      guard (int_typed (size_of Γ τ) sptrT);
-     '(e,τ') ← to_R <$> to_expr Γ ∅ m ((x,inr τ) :: xs) ce;
+     '(e,τ') ← to_R <$> to_expr Γn Γ ∅ m ((x,inr τ) :: xs) ce;
      guard (τ = τ');
      '(m,s,cmσ) ← go m ((x,inr τ) :: xs) Ls mLc mLb cs;
      Some (m, blk{τ} (var{τ} 0 ::= e ;; s), cmσ)
   | SStatic x τ mce cs =>
-     '(m,xs) ← alloc_global Γ m xs x τ mce;
+     '(m,xs) ← alloc_global Γn Γ m xs x τ mce;
      go m xs Ls mLc mLb cs
   | SComp cs1 cs2 =>
      '(m,s1,cmσ1) ← go m xs Ls mLc mLb cs1;
@@ -289,38 +299,42 @@ Definition to_stmt (Γ : env Ti) (Γf : funtypes Ti) :
   | SLabel l cs =>
      '(m,s,cmσ) ← go m xs Ls mLc mLb cs; Some (m, l :; s, cmσ)
   | SWhile ce cs =>
-     '(e,τ) ← to_R <$> to_expr Γ Γf m xs ce; _ ← maybe_TBase τ;
+     '(e,τ) ← to_R <$> to_expr Γn Γ Γf m xs ce; _ ← maybe_TBase τ;
      let '(Ls,mLc,mLb,Fs) :=
        to_while e (cstmt_has_continue cs) (cstmt_has_break cs) Ls in
      '(m,s,cmσ) ← go m xs Ls mLc mLb cs;
      Some (m, Fs s, (false, cmσ.2))
   | SIf ce cs1 cs2 =>
-     '(e,τ) ← to_R <$> to_expr Γ Γf m xs ce; _ ← maybe_TBase τ;
+     '(e,τ) ← to_R <$> to_expr Γn Γ Γf m xs ce; _ ← maybe_TBase τ;
      '(m,s1,cmσ1) ← go m xs Ls mLc mLb cs1;
      '(m,s2,cmσ2) ← go m xs Ls mLc mLb cs2;
      mσ ← rettype_union (cmσ1.2) (cmσ2.2);
      Some (m, if{e} s1 else s2, (cmσ1.1 && cmσ2.1, mσ))%S
   end%T.
 
-Fixpoint to_envs (Θ : list (N * decl Ti)) :
-    option (env Ti * funtypes Ti * funenv Ti * mem Ti * var_env Ti) :=
+Fixpoint to_envs (Θ : list (N * decl Ti)) : option
+    (rename_env * env Ti * funtypes Ti * funenv Ti * mem Ti * var_env Ti) :=
   match Θ with
-  | [] => Some (∅,∅,∅,∅,[])
-  | (s,CompoundDecl τs) :: Θ =>
-     '(Γ,Γf,δ,m,xs) ← to_envs Θ;
+  | [] => Some (∅,∅,∅,∅,∅,[])
+  | (s,CompoundDecl τys) :: Θ =>
+     (* todo: names of structures and unions should not collapse *)
+     '(Γn,Γ,Γf,δ,m,xs) ← to_envs Θ;
      let s : tag := s in
+     let ys := fst <$> τys in
+     let τs := snd <$> τys in
      guard (Γ !! s = None);
+     guard (NoDup ys);
      guard (✓{Γ}* τs);
      guard (1 < length τs);
-     Some (<[s:=τs]>Γ, Γf, δ, m, xs)
+     Some (<[s:=ys]>Γn, <[s:=τs]>Γ, Γf, δ, m, xs)
   | (x,GlobDecl τ me) :: Θ =>
      (* todo: we just shadow, that is wrong *)
-     '(Γ,Γf,δ,m,xs) ← to_envs Θ;
-     '(m,xs) ← alloc_global Γ m xs x τ me;
-      Some (Γ, Γf, δ, m, xs)
+     '(Γn,Γ,Γf,δ,m,xs) ← to_envs Θ;
+     '(m,xs) ← alloc_global Γn Γ m xs x τ me;
+      Some (Γn, Γ, Γf, δ, m, xs)
   | (f,FunDecl ys σ cs) :: Θ =>
      (* todo: functions and globals cannot have the same name *)
-     '(Γ,Γf,δ,m,xs) ← to_envs Θ;
+     '(Γn,Γ,Γf,δ,m,xs) ← to_envs Θ;
      let f : funname := f in
      guard (NoDup (fst <$> ys));
      let τs := snd <$> ys in
@@ -328,9 +342,9 @@ Fixpoint to_envs (Θ : list (N * decl Ti)) :
      guard (✓{Γ}* τs);
      guard (Forall (λ τ, int_typed (size_of Γ τ) sptrT) τs);
      let xs' := (prod_map id inr <$> ys) ++ xs in
-     '(m,s,cmσ) ← to_stmt Γ Γf m xs' (labels cs) None None cs;
+     '(m,s,cmσ) ← to_stmt Γn Γ Γf m xs' (labels cs) None None cs;
      guard (rettype_match cmσ σ);
-     Some(Γ, <[f:=(τs,σ)]>Γf, <[f:=s]>δ, m, xs)
+     Some(Γn, Γ, <[f:=(τs,σ)]>Γf, <[f:=s]>δ, m, xs)
   end.
 End frontend.
 
@@ -433,21 +447,20 @@ Proof.
   * rewrite cons_middle, (associative_L (++)). apply (IH (τs' ++ [τ'])).
     rewrite app_length; simpl. by rewrite Nat.add_comm.
 Qed.
-Lemma to_expr_typed Γ Γf m xs ce e τlr :
-  ✓ Γ → ✓{Γ} m → to_expr Γ Γf m xs ce = Some (e,τlr) →
+Lemma to_expr_typed Γn Γ Γf m xs ce e τlr :
+  ✓ Γ → ✓{Γ} m → to_expr Γn Γ Γf m xs ce = Some (e,τlr) →
   (Γ,Γf,m,var_env_stack_types xs) ⊢ e : τlr.
 Proof.
   intros ??. assert (∀ ces eτlrs,
-     Forall (λ ce, ∀ e τlr, to_expr Γ Γf m xs ce = Some (e,τlr) →
+     Forall (λ ce, ∀ e τlr, to_expr Γn Γ Γf m xs ce = Some (e,τlr) →
        (Γ,Γf,m,var_env_stack_types xs) ⊢ e : τlr) ces →
-     mapM (to_expr Γ Γf m xs) ces = Some eτlrs →
+     mapM (to_expr Γn Γ Γf m xs) ces = Some eτlrs →
      (Γ,Γf,m,var_env_stack_types xs) ⊢*
        fst <$> to_R <$> eτlrs :* inr <$> snd <$> to_R <$> eτlrs).
   { intros ces eτlrs. rewrite mapM_Some. induction 2 as [|? [??]];
-      decompose_Forall_hyps'; eauto using to_R_typed, surjective_pairing. }
+      decompose_Forall_hyps; eauto using to_R_typed, surjective_pairing. }
   revert e τlr. induction ce using @cexpr_ind_alt; intros;
     repeat match goal with
-    | _ => progress case_match
     | _ : maybe_inl ?τlr = Some _ |- _ => is_var τlr; destruct τlr
     | _ : maybe_TBase ?τ = Some _ |- _ => is_var τ; destruct τ
     | _ : maybe_TPtr ?τb = Some _ |- _ => is_var τb; destruct τb
@@ -457,19 +470,20 @@ Proof.
     | H: unop_type_of _ _ = Some _ |- _ => apply unop_type_of_correct in H
     | H: binop_type_of _ _ _ = Some _ |- _ => apply binop_type_of_correct in H
     | _ => progress (simplify_option_equality by fail)
+    | _ => progress case_match
     | x : (_ * _)%type |- _ => destruct x
     end; repeat typed_constructor;
     eauto using to_R_typed, var_lookup_typed, ECasts_typed.
 Qed.
-Lemma alloc_global_typed Γ m xs x τ mce m' xs' :
-  ✓ Γ → alloc_global Γ m xs x τ mce = Some (m',xs') →
+Lemma alloc_global_typed Γn Γ m xs x τ mce m' xs' :
+  ✓ Γ → alloc_global Γn Γ m xs x τ mce = Some (m',xs') →
   ✓{Γ} m → ✓{Γ} m' ∧ (∀ o σ, m ⊢ o : σ → m' ⊢ o : σ)
     ∧ var_env_stack_types xs = var_env_stack_types xs'.
 Proof.
   assert (mem_allocable (fresh (dom indexset m)) m).
   { eapply mem_allocable_alt, is_fresh. }
   destruct mce as [ce|]; intros; simplify_equality'.
-  * destruct (to_expr Γ ∅ m xs ce) as [[e τlr]|] eqn:?; simplify_equality'.
+  * destruct (to_expr Γn Γ ∅ m xs ce) as [[e τlr]|] eqn:?; simplify_equality'.
     destruct (to_R (e, τlr)) as [e' τ'] eqn:?.
     repeat case_option_guard; simplify_equality'.
     destruct (⟦ e' ⟧ Γ ∅ [] m) as [[?|v]|] eqn:?; simplify_equality'.
@@ -489,8 +503,8 @@ Proof.
   destruct con, bre; intros; simplify_equality';
     repeat typed_constructor; eauto using rettype_union_l.
 Qed.
-Lemma to_stmt_typed Γ Γf m xs Ls mLc mLb cs m' s cmτ :
-  ✓ Γ → ✓{Γ} m → to_stmt Γ Γf m xs Ls mLc mLb cs = Some (m',s,cmτ) →
+Lemma to_stmt_typed Γn Γ Γf m xs Ls mLc mLb cs m' s cmτ :
+  ✓ Γ → ✓{Γ} m → to_stmt Γn Γ Γf m xs Ls mLc mLb cs = Some (m',s,cmτ) →
   (Γ,Γf,m',var_env_stack_types xs) ⊢ s : cmτ
   ∧ ✓{Γ} m' ∧ (∀ o σ, m ⊢ o : σ → m' ⊢ o : σ).
 Proof.
@@ -500,13 +514,13 @@ Proof.
     | _ : maybe_TBase ?τ = Some _ |- _ => is_var τ; destruct τ
     | _ => progress (simplify_option_equality by fail)
     | x : (_ * _)%type |- _ => destruct x
-    | IH : ∀ _ _ _ _ _ _ _ _, ✓{Γ} _ → to_stmt _ _ _ _ _ _ _ ?cs = Some _ → _,
-      H : to_stmt _ _ _ _ _ _ _ ?cs = Some _ |- _ =>
+    | IH : ∀ _ _ _ _ _ _ _ _, ✓{Γ} _ → to_stmt _ _ _ _ _ _ _ _ ?cs = Some _ → _,
+      H : to_stmt _ _ _ _ _ _ _ _ ?cs = Some _ |- _ =>
        destruct (λ Hm, IH _ _ _ _ _ _ _ _ Hm H) as (?&?&?); clear IH; [by auto|]
-    | H : to_expr _ _ _ _ _ = Some _ |- _ =>
+    | H : to_expr _ _ _ _ _ _ = Some _ |- _ =>
        apply to_expr_typed in H; [|by auto|by auto];
        eapply to_R_typed in H; [|by eauto]
-    | H : alloc_global _ _ _ _ _ _ = Some _ |- _ =>
+    | H : alloc_global _ _ _ _ _ _ _ = Some _ |- _ =>
        apply alloc_global_typed in H; [|by auto|by auto]; destruct H as (?&?&->)
     end; try solve [split_ands; eauto using to_R_typed, to_expr_typed].
   * split_ands; eauto. eapply SBlock_typed; eauto.
@@ -516,29 +530,29 @@ Proof.
   * split_ands; eauto using to_while_typed, expr_typed_weaken.
   * split_ands; eauto using stmt_typed_weaken, expr_typed_weaken.
 Qed.
-Lemma to_envs_typed Θ Γ Γf δ m xs :
-  to_envs Θ = Some (Γ,Γf,δ,m,xs) →
+Lemma to_envs_typed Θ Γn Γ Γf δ m xs :
+  to_envs Θ = Some (Γn,Γ,Γf,δ,m,xs) →
   ✓ Γ ∧ (Γ,m) ⊢ δ : Γf ∧ ✓{Γ} m ∧ var_env_stack_types xs = [].
 Proof.
-  revert Γ Γf δ m xs. induction Θ as [|[x [τs|τ mce|ys σ cs]] Θ IH];
-    intros Γ Γf δ m xs ?; simplify_equality'.
+  revert Γn Γ Γf δ m xs. induction Θ as [|[x [τs|τ mce|ys σ cs]] Θ IH];
+    intros Γn Γ Γf δ m xs ?; simplify_equality'.
   * eauto using env_empty_valid, cmap_empty_valid.
-  * destruct (to_envs Θ) as [[[[[Γ2 ?] ?] ?] ?]|]; simplify_option_equality.
-    destruct (IH Γ2 Γf δ m xs) as (?&?&?&?); eauto. split_ands; auto.
+  * destruct (to_envs Θ) as [[[[[[Γn2 Γ2] ?] ?] ?] ?]|]; simplify_option_equality.
+    destruct (IH Γn2 Γ2 Γf δ m xs) as (?&?&?&?); eauto. split_ands; auto.
     + by constructor.
     + eapply funenv_typed_weaken; eauto using insert_subseteq.
     + eapply cmap_valid_weaken; eauto using insert_subseteq.
-  * destruct (to_envs Θ) as [[[[[Γ2 Γf2] δ2] m2] xs2]|]; simplify_equality'.
-    destruct (alloc_global _ _ _ _ _ _) as [[??]|] eqn:?; simplify_equality'.
-    destruct (IH Γ Γf δ m2 xs2) as (?&?&?&?); eauto.
-    destruct (alloc_global_typed Γ m2 xs2 x τ mce m xs)
+  * destruct (to_envs Θ) as [[[[[[Γn2 Γ2] Γf2] δ2] m2] xs2]|]; simplify_equality'.
+    destruct (alloc_global _ _ _ _ _ _ _) as [[??]|] eqn:?; simplify_equality'.
+    destruct (IH Γn Γ Γf δ m2 xs2) as (?&?&?&?); eauto.
+    destruct (alloc_global_typed Γn Γ m2 xs2 x τ mce m xs)
       as (?&?&<-); eauto using funenv_typed_weaken.
-  * destruct (to_envs Θ) as [[[[[Γ2 Γf2] δ2] m2] xs2]|]; simplify_equality'.
+  * destruct (to_envs Θ) as [[[[[[Γn2 Γ2] Γf2] δ2] m2] xs2]|]; simplify_equality'.
     repeat case_option_guard; simplify_equality'.
-    destruct (to_stmt _ _ _ _ _ _ _ _)
+    destruct (to_stmt _ _ _ _ _ _ _ _ _)
       as [[[m3 s] cmσ]|] eqn:?; simplify_option_equality.
-    destruct (IH Γ Γf2 δ2 m2 xs) as (?&?&?&Hxs); eauto.
-    destruct (to_stmt_typed Γ Γf2 m2 ((prod_map id inr <$> ys) ++ xs)
+    destruct (IH Γn Γ Γf2 δ2 m2 xs) as (?&?&?&Hxs); eauto.
+    destruct (to_stmt_typed Γn Γ Γf2 m2 ((prod_map id inr <$> ys) ++ xs)
       (labels cs) None None cs m s cmσ) as (Hs&?&?); auto.
     rewrite var_env_stack_types_app,
       var_env_stack_types_snd, Hxs, (right_id_L [] (++)) in Hs.
